Spec.QUIC -> QUIC.Spec; Impl.QUIC -> QUIC.Impl

src/QUIC.Impl.fst
@@ -1,6 +1,6 @@
-module Impl.QUIC
+module QUIC.Impl
 
-// This MUST be kept in sync with Impl.QUIC.fsti...
+// This MUST be kept in sync with QUIC.Impl.fsti...
 module G = FStar.Ghost
 module B = LowStar.Buffer
 module IB = LowStar.ImmutableBuffer
@@ -27,12 +27,12 @@ module AEAD = EverCrypt.AEAD
 module HKDF = EverCrypt.HKDF
 module CTR = EverCrypt.CTR
 
-friend Spec.QUIC
+friend QUIC.Spec
 
 open LowStar.BufferOps
 
 inline_for_extraction noextract
-let as_cipher_alg (a: Spec.QUIC.ea) =
+let as_cipher_alg (a: QUIC.Spec.ea) =
   Spec.Agile.AEAD.cipher_alg_of_supported_alg a
 
 /// https://tools.ietf.org/html/draft-ietf-quic-tls-23#section-5
@@ -50,10 +50,10 @@ type state_s (i: index) =
       the_hash_alg:hash_alg { the_hash_alg == i.hash_alg } ->
       the_aead_alg:aead_alg { the_aead_alg == i.aead_alg } ->
       traffic_secret:G.erased (Spec.Hash.Definitions.bytes_hash the_hash_alg) ->
-      initial_pn:G.erased Spec.QUIC.nat62 ->
+      initial_pn:G.erased QUIC.Spec.nat62 ->
       aead_state:EverCrypt.AEAD.state the_aead_alg ->
       iv:EverCrypt.AEAD.iv_p the_aead_alg ->
-      hp_key:B.buffer U8.t { B.length hp_key = Spec.QUIC.ae_keysize the_aead_alg } ->
+      hp_key:B.buffer U8.t { B.length hp_key = QUIC.Spec.ae_keysize the_aead_alg } ->
       pn:B.pointer u62 ->
       ctr_state:CTR.state (as_cipher_alg the_aead_alg) ->
       state_s i
@@ -75,7 +75,7 @@ let g_initial_packet_number #i s =
   State?.initial_pn s
 
 let invariant_s #i h s =
-  let open Spec.QUIC in
+  let open QUIC.Spec in
   let State hash_alg aead_alg traffic_secret initial_pn aead_state iv hp_key pn ctr_state =
     s
   in
@@ -92,7 +92,7 @@ let invariant_s #i h s =
   B.as_seq h iv ==
     derive_secret i.hash_alg (G.reveal traffic_secret) label_iv 12 /\
   B.as_seq h hp_key ==
-    derive_secret i.hash_alg (G.reveal traffic_secret) label_hp (Spec.QUIC.ae_keysize aead_alg)
+    derive_secret i.hash_alg (G.reveal traffic_secret) label_hp (QUIC.Spec.ae_keysize aead_alg)
   )
 
 let invariant_loc_in_footprint #_ _ _ = ()
@@ -123,7 +123,7 @@ let packet_number_of_state #i s =
 /// are UInt32's, mostly to avoid trouble reasoning with modulo when casting
 /// from UInt32 to UInt8 to write the label for the key derivation. This could
 /// be fixed later.
-val derive_secret: a: Spec.QUIC.ha ->
+val derive_secret: a: QUIC.Spec.ha ->
   dst:B.buffer U8.t ->
   dst_len: U8.t { B.length dst = U8.v dst_len /\ U8.v dst_len <= 255 } ->
   secret:B.buffer U8.t { B.length secret = Spec.Hash.Definitions.hash_length a } ->
@@ -137,11 +137,11 @@ val derive_secret: a: Spec.QUIC.ha ->
       assert_norm (255 < pow2 61);
       assert_norm (pow2 61 < pow2 125);
       B.(modifies (loc_buffer dst) h0 h1) /\
-      B.as_seq h1 dst == Spec.QUIC.derive_secret a (B.as_seq h0 secret)
+      B.as_seq h1 dst == QUIC.Spec.derive_secret a (B.as_seq h0 secret)
         (IB.as_seq h0 label) (U8.v dst_len))
 #pop-options
 
-let prefix = LowStar.ImmutableBuffer.igcmalloc_of_list HS.root Spec.QUIC.prefix_l
+let prefix = LowStar.ImmutableBuffer.igcmalloc_of_list HS.root QUIC.Spec.prefix_l
 
 let lemma_five_cuts (s: S.seq U8.t) (i1 i2 i3 i4 i5: nat) (s0 s1 s2 s3 s4 s5: S.seq U8.t): Lemma
   (requires (
@@ -166,8 +166,8 @@ let lemma_five_cuts (s: S.seq U8.t) (i1 i2 i3 i4 i5: nat) (s0 s1 s2 s3 s4 s5: S.
 =
   ()
 
-let hash_is_keysized_ (a: Spec.QUIC.ha): Lemma
-  (ensures (Spec.QUIC.keysized a (Spec.Hash.Definitions.hash_length a)))
+let hash_is_keysized_ (a: QUIC.Spec.ha): Lemma
+  (ensures (QUIC.Spec.keysized a (Spec.Hash.Definitions.hash_length a)))
 =
   assert_norm (512 < pow2 61);
   assert_norm (512 < pow2 125)
@@ -175,7 +175,7 @@ let hash_is_keysized_ (a: Spec.QUIC.ha): Lemma
 #set-options "--z3rlimit 100"
 let derive_secret a dst dst_len secret label label_len =
   LowStar.ImmutableBuffer.recall prefix;
-  LowStar.ImmutableBuffer.recall_contents prefix Spec.QUIC.prefix;
+  LowStar.ImmutableBuffer.recall_contents prefix QUIC.Spec.prefix;
   (**) let h0 = ST.get () in
 
   push_frame ();
@@ -211,7 +211,7 @@ let derive_secret a dst dst_len secret label label_len =
   (**)   B.as_seq h2 info_z `Seq.equal` z /\
   (**)   B.as_seq h2 info_lb `Seq.equal` lb /\
   (**)   B.as_seq h2 info_llen `Seq.equal` llen /\
-  (**)   B.as_seq h2 info_prefix `Seq.equal` Spec.QUIC.prefix /\
+  (**)   B.as_seq h2 info_prefix `Seq.equal` QUIC.Spec.prefix /\
   (**)   B.as_seq h2 info_label `Seq.equal` (B.as_seq h0 label) /\
   (**)   B.as_seq h2 info_z' `Seq.equal` z
   (**) );
@@ -221,7 +221,7 @@ let derive_secret a dst dst_len secret label label_len =
   (**)   let llen = S.create 1 (U8.uint_to_t (11 + Seq.length (B.as_seq h0 label))) in
   (**)   let info = B.as_seq h2 info in
   (**)   lemma_five_cuts info 1 2 3 14 (14 + U8.v label_len)
-  (**)     z lb llen Spec.QUIC.prefix (B.as_seq h0 label) z
+  (**)     z lb llen QUIC.Spec.prefix (B.as_seq h0 label) z
   (**) );
   (**) hash_is_keysized_ a;
   HKDF.expand a dst secret (Hacl.Hash.Definitions.hash_len a) info info_len dst_len32;
@@ -231,7 +231,7 @@ let derive_secret a dst dst_len secret label label_len =
   (**) B.modifies_fresh_frame_popped h0 h1 (B.loc_buffer dst) h3 h4;
   (**) assert (ST.equal_domains h0 h4)
 
-let key_len (a: Spec.QUIC.ea): x:U8.t { U8.v x = Spec.Agile.AEAD.key_length a } =
+let key_len (a: QUIC.Spec.ea): x:U8.t { U8.v x = Spec.Agile.AEAD.key_length a } =
   let open Spec.Agile.AEAD in
   match a with
   | AES128_GCM -> 16uy
@@ -240,26 +240,26 @@ let key_len (a: Spec.QUIC.ea): x:U8.t { U8.v x = Spec.Agile.AEAD.key_length a } 
 
 let key_len32 a = FStar.Int.Cast.uint8_to_uint32 (key_len a)
 
-let label_key = LowStar.ImmutableBuffer.igcmalloc_of_list HS.root Spec.QUIC.label_key_l
-let label_iv = LowStar.ImmutableBuffer.igcmalloc_of_list HS.root Spec.QUIC.label_iv_l
-let label_hp = LowStar.ImmutableBuffer.igcmalloc_of_list HS.root Spec.QUIC.label_hp_l
+let label_key = LowStar.ImmutableBuffer.igcmalloc_of_list HS.root QUIC.Spec.label_key_l
+let label_iv = LowStar.ImmutableBuffer.igcmalloc_of_list HS.root QUIC.Spec.label_iv_l
+let label_hp = LowStar.ImmutableBuffer.igcmalloc_of_list HS.root QUIC.Spec.label_hp_l
 
 // JP: this proof currently takes 12 minutes. It could conceivably be improved.
 #push-options "--z3rlimit 1000 --query_stats"
 let create_in i r dst initial_pn traffic_secret =
   LowStar.ImmutableBuffer.recall label_key;
-  LowStar.ImmutableBuffer.recall_contents label_key Spec.QUIC.label_key;
+  LowStar.ImmutableBuffer.recall_contents label_key QUIC.Spec.label_key;
   LowStar.ImmutableBuffer.recall label_iv;
-  LowStar.ImmutableBuffer.recall_contents label_iv Spec.QUIC.label_iv;
+  LowStar.ImmutableBuffer.recall_contents label_iv QUIC.Spec.label_iv;
   LowStar.ImmutableBuffer.recall label_hp;
-  LowStar.ImmutableBuffer.recall_contents label_hp Spec.QUIC.label_hp;
+  LowStar.ImmutableBuffer.recall_contents label_hp QUIC.Spec.label_hp;
   (**) let h0 = ST.get () in
   [@inline_let]
   let e_traffic_secret: G.erased (Spec.Hash.Definitions.bytes_hash i.hash_alg) =
     G.hide (B.as_seq h0 traffic_secret)
   in
   [@inline_let]
-  let e_initial_pn: G.erased Spec.QUIC.nat62 = G.hide (U64.v initial_pn) in
+  let e_initial_pn: G.erased QUIC.Spec.nat62 = G.hide (U64.v initial_pn) in
   [@inline_let]
   let hash_alg = i.hash_alg in
   [@inline_let]
@@ -323,7 +323,7 @@ let create_in i r dst initial_pn traffic_secret =
       (**) let h6 = ST.get () in
       (**) B.(modifies_loc_includes (loc_buffer dst) h5 h6 loc_none);
 
-      (**) assert (B.length hp_key = Spec.QUIC.ae_keysize aead_alg);
+      (**) assert (B.length hp_key = QUIC.Spec.ae_keysize aead_alg);
       let s: state_s i = State #i
         hash_alg aead_alg e_traffic_secret e_initial_pn
         aead_state iv hp_key pn ctr_state
@@ -375,52 +375,52 @@ let lemma_slice s (i: nat { i <= S.length s }): Lemma
 #set-options "--max_fuel 1 --z3rlimit 100"
 let rec pointwise_upd (#a: eqtype) f b1 b2 i pos (x: a): Lemma
   (requires (S.length b2 + pos <= S.length b1 /\ i < pos))
-  (ensures (S.upd (Spec.QUIC.pointwise_op f b1 b2 pos) i x `S.equal`
-    Spec.QUIC.pointwise_op f (S.upd b1 i x) b2 pos))
+  (ensures (S.upd (QUIC.Spec.pointwise_op f b1 b2 pos) i x `S.equal`
+    QUIC.Spec.pointwise_op f (S.upd b1 i x) b2 pos))
   (decreases (S.length b2))
 =
   calc (S.equal) {
-    Spec.QUIC.pointwise_op f (S.upd b1 i x) b2 pos;
+    QUIC.Spec.pointwise_op f (S.upd b1 i x) b2 pos;
   (S.equal) { lemma_slice (S.upd b1 i x) (i + 1) }
-    Spec.QUIC.pointwise_op f
+    QUIC.Spec.pointwise_op f
       S.(slice (S.upd b1 i x) 0 (i + 1) @| S.slice (S.upd b1 i x) (i + 1) (S.length b1))
       b2 pos;
   (S.equal) { }
-    Spec.QUIC.pointwise_op f
+    QUIC.Spec.pointwise_op f
       S.(slice (S.upd b1 i x) 0 (i + 1) @| S.slice b1 (i + 1) (S.length b1))
       b2 pos;
   (S.equal) {
-    Spec.QUIC.pointwise_op_suff f
+    QUIC.Spec.pointwise_op_suff f
       (S.slice (S.upd b1 i x) 0 (i + 1))
       (S.slice b1 (i + 1) (S.length b1)) b2 pos
   }
     S.slice (S.upd b1 i x) 0 (i + 1) `S.append`
-    Spec.QUIC.pointwise_op f
+    QUIC.Spec.pointwise_op f
       (S.slice b1 (i + 1) (S.length b1))
       b2 (pos - (i + 1));
   (S.equal) { }
     S.upd (S.slice b1 0 (i + 1)) i x `S.append`
-    Spec.QUIC.pointwise_op f
+    QUIC.Spec.pointwise_op f
       (S.slice b1 (i + 1) (S.length b1))
       b2 (pos - (i + 1));
   (S.equal) { }
     S.upd (S.slice b1 0 (i + 1) `S.append`
-    Spec.QUIC.pointwise_op f
+    QUIC.Spec.pointwise_op f
       (S.slice b1 (i + 1) (S.length b1))
       b2 (pos - (i + 1))
     ) i x;
   (S.equal) {
-    Spec.QUIC.pointwise_op_suff f
+    QUIC.Spec.pointwise_op_suff f
       (S.slice b1 0 (i + 1))
       (S.slice b1 (i + 1) (S.length b1)) b2 pos
   }
     S.upd (
-      Spec.QUIC.pointwise_op f
+      QUIC.Spec.pointwise_op f
       (S.slice b1 0 (i + 1) `S.append` S.slice b1 (i + 1) (S.length b1))
       b2 pos
     ) i x;
   (S.equal) { lemma_slice b1 (i + 1) }
-    S.upd (Spec.QUIC.pointwise_op f b1 b2 pos) i x;
+    S.upd (QUIC.Spec.pointwise_op f b1 b2 pos) i x;
   }
 
 #push-options "--z3rlimit 50"
@@ -431,7 +431,7 @@ let rec pointwise_seq_map2 (#a: eqtype) (f: a -> a -> a) (s1 s2: S.seq a) (i: na
   (ensures (
     let l = S.length s1 in
     Spec.Loops.seq_map2 f (S.slice s1 i l) s2 `S.equal`
-    S.slice (Spec.QUIC.pointwise_op f s1 s2 i) i l))
+    S.slice (QUIC.Spec.pointwise_op f s1 s2 i) i l))
   (decreases (S.length s2))
 =
   if S.length s2 = 0 then
@@ -448,17 +448,17 @@ let rec pointwise_seq_map2 (#a: eqtype) (f: a -> a -> a) (s1 s2: S.seq a) (i: na
         (Spec.Loops.seq_map2 f (S.slice s1 (i + 1) l) (S.tail s2));
     (S.equal) { pointwise_seq_map2 f s1 (S.slice s2 1 (S.length s2)) (i + 1) }
       S.cons (f (S.head (S.slice s1 i l)) (S.head s2))
-        (S.slice (Spec.QUIC.pointwise_op f s1 (S.tail s2) (i + 1)) (i + 1) l);
+        (S.slice (QUIC.Spec.pointwise_op f s1 (S.tail s2) (i + 1)) (i + 1) l);
     (S.equal) { }
       S.slice (
-        S.upd (Spec.QUIC.pointwise_op f s1 (S.tail s2) (i + 1))
+        S.upd (QUIC.Spec.pointwise_op f s1 (S.tail s2) (i + 1))
           i
           (f (S.head (S.slice s1 i l)) (S.head s2)))
         i
         l;
     (S.equal) { }
       S.slice (
-        S.upd (Spec.QUIC.pointwise_op f s1 (S.slice s2 1 (S.length s2)) (i + 1))
+        S.upd (QUIC.Spec.pointwise_op f s1 (S.slice s2 1 (S.length s2)) (i + 1))
           i
           (f (S.head (S.slice s1 i l)) (S.head s2)))
         i
@@ -468,7 +468,7 @@ let rec pointwise_seq_map2 (#a: eqtype) (f: a -> a -> a) (s1 s2: S.seq a) (i: na
         (f (S.head (S.slice s1 i l)) (S.head s2))
     }
       S.slice
-        (Spec.QUIC.pointwise_op f
+        (QUIC.Spec.pointwise_op f
           (S.upd s1 i (f (S.head (S.slice s1 i l)) (S.head s2)))
           (S.slice s2 1 (S.length s2))
           (i + 1))
@@ -493,7 +493,7 @@ let op_inplace (dst src: B.buffer U8.t)
     (ensures fun h0 _ h1 ->
       B.(modifies (loc_buffer dst) h0 h1) /\
       B.as_seq h1 dst `S.equal`
-        Spec.QUIC.pointwise_op op (B.as_seq h0 dst) (B.as_seq h0 src) (U32.v ofs))
+        QUIC.Spec.pointwise_op op (B.as_seq h0 dst) (B.as_seq h0 src) (U32.v ofs))
 =
   let h0 = ST.get () in
   let dst0 = B.sub dst 0ul ofs in
@@ -513,22 +513,22 @@ let op_inplace (dst src: B.buffer U8.t)
       (S.slice (B.as_seq h1 dst) (U32.v ofs) (B.length dst));
   (S.equal) { pointwise_seq_map2 op (B.as_seq h0 dst') (B.as_seq h0 src) 0 }
     S.append (S.slice (B.as_seq h0 dst) 0 (U32.v ofs))
-      (Spec.QUIC.pointwise_op op
+      (QUIC.Spec.pointwise_op op
         (S.slice (B.as_seq h0 dst) (U32.v ofs) (B.length dst))
         (B.as_seq h0 src)
         0);
-  (S.equal) { Spec.QUIC.pointwise_op_suff op (S.slice (B.as_seq h0 dst) 0 (U32.v ofs))
+  (S.equal) { QUIC.Spec.pointwise_op_suff op (S.slice (B.as_seq h0 dst) 0 (U32.v ofs))
     (S.slice (B.as_seq h0 dst) (U32.v ofs) (B.length dst))
     (B.as_seq h0 src)
     (U32.v ofs)
   }
-    Spec.QUIC.pointwise_op op
+    QUIC.Spec.pointwise_op op
       (S.append (S.slice (B.as_seq h0 dst) 0 (U32.v ofs))
         (S.slice (B.as_seq h0 dst) (U32.v ofs) (B.length dst)))
       (B.as_seq h0 src)
       (U32.v ofs);
   (S.equal) { lemma_slice (B.as_seq h0 dst) (U32.v ofs) }
-    Spec.QUIC.pointwise_op op
+    QUIC.Spec.pointwise_op op
       (B.as_seq h0 dst)
       (B.as_seq h0 src)
       (U32.v ofs);
@@ -549,20 +549,20 @@ let header_disjoint (h: header) =
 let format_header (dst: B.buffer U8.t) (h: header) (npn: B.buffer U8.t) (pn_len: u2):
   Stack unit
     (requires (fun h0 ->
-      B.length dst = Spec.QUIC.header_len (g_header h h0) (U8.v pn_len) /\
+      B.length dst = QUIC.Spec.header_len (g_header h h0) (U8.v pn_len) /\
       B.length npn = 1 + U8.v pn_len /\
       header_live h h0 /\
       header_disjoint h /\
       B.(all_disjoint [ loc_buffer dst; header_footprint h; loc_buffer npn ])))
     (ensures (fun h0 _ h1 ->
       B.(modifies (loc_buffer dst) h0 h1) /\ (
-      let fh = Spec.QUIC.format_header (g_header h h0) (B.as_seq h0 npn) in
+      let fh = QUIC.Spec.format_header (g_header h h0) (B.as_seq h0 npn) in
       S.slice (B.as_seq h1 dst) 0 (S.length fh) `S.equal` fh)))
 =
   admit ();
   C.Failure.failwith C.String.(!$"TODO")
 
-let vlen (n:u62) : x:U8.t { U8.v x = Spec.QUIC.vlen (U64.v n) } =
+let vlen (n:u62) : x:U8.t { U8.v x = QUIC.Spec.vlen (U64.v n) } =
   assert_norm (pow2 6 = 64);
   assert_norm (pow2 14 = 16384);
   assert_norm (pow2 30 = 1073741824);
@@ -574,7 +574,7 @@ let vlen (n:u62) : x:U8.t { U8.v x = Spec.QUIC.vlen (U64.v n) } =
 let header_len (h: header) (pn_len: u2): Stack U32.t
   (requires fun h0 -> True)
   (ensures fun h0 x h1 ->
-    U32.v x = Spec.QUIC.header_len (g_header h h0) (U8.v pn_len) /\
+    U32.v x = QUIC.Spec.header_len (g_header h h0) (U8.v pn_len) /\
     h0 == h1)
 =
   [@inline_let]
@@ -634,7 +634,7 @@ let block_of_sample (a: Spec.Agile.Cipher.cipher_alg)
     (ensures fun h0 _ h1 ->
       B.(modifies (loc_buffer dst `loc_union` CTR.footprint h0 s) h0 h1) /\
       B.as_seq h1 dst `S.equal`
-        Spec.QUIC.block_of_sample a (B.as_seq h0 k) (B.as_seq h0 sample))
+        QUIC.Spec.block_of_sample a (B.as_seq h0 k) (B.as_seq h0 sample))
 =
   push_frame ();
   (**) let h0 = ST.get () in
@@ -685,7 +685,7 @@ let encrypt #i s dst h plain plain_len pn_len =
   (**) let h0 = ST.get () in
   assert (
     let s0 = g_traffic_secret (B.deref h0 s) in
-    let open Spec.QUIC in
+    let open QUIC.Spec in
     let k = derive_secret i.hash_alg s0 label_key (Spec.Agile.AEAD.key_length i.aead_alg) in
     let iv_seq = derive_secret i.hash_alg s0 label_iv 12 in
     let hp_key_seq = derive_secret i.hash_alg s0 label_hp (ae_keysize i.aead_alg) in
